adequacy

theories/ghost_state.v
@@ -4,34 +4,59 @@ From iris.algebra Require Import big_op gmap frac agree.
 From iris.algebra Require Import csum excl auth cmra_big_op numbers.
 From iris.bi Require Import fractional.
 From iris.base_logic Require Export lib.own.
-From iris.base_logic.lib Require Import ghost_map.
+From iris.base_logic.lib Require Import ghost_map ghost_var.
 From iris.proofmode Require Export tactics.
 From isla Require Export opsem.
 Set Default Proof Using "Type".
 Import uPred.
 
+Definition instrtblUR : cmra :=
+  agreeR (gmapO addr (leibnizO (list trc))).
+
+
 Class heapG Σ := HeapG {
-  heap_instrs_inG :> ghost_mapG Σ addr (list trc);
+  heap_instrs_inG :> inG Σ instrtblUR;
   heap_instrs_name : gname;
   heap_regs_inG :> ghost_mapG Σ string valu;
+  heap_full_trace : list seq_label;
+  heap_spec_trace : list seq_label;
+  heap_spec_trace_inG :> ghost_varG Σ (list seq_label);
+  heap_spec_trace_name : gname;
 }.
 
 Class threadG := ThreadG {
   thread_regs_name : gname;
 }.
 
+Definition to_instrtbl : gmap addr (list trc) → instrtblUR :=
+  to_agree.
+
 Section definitions.
   Context `{!heapG Σ}.
 
-  Definition instr_def (a : addr) (i: list trc) : iProp Σ :=
-    a ↪[ heap_instrs_name ]□ i.
+  Definition instr_table_def (i : gmap addr (list trc)) : iProp Σ :=
+    own heap_instrs_name (to_instrtbl i).
+  Definition instr_table_aux : seal (@instr_table_def). by eexists. Qed.
+  Definition instr_table := unseal instr_table_aux.
+  Definition instr_table_eq : @instr_table = @instr_table_def :=
+    seal_eq instr_table_aux.
+
+  Definition instr_def (a : addr) (i: option (list trc)) : iProp Σ :=
+    ∃ instrs, ⌜instrs !! a = i⌝ ∗ instr_table instrs.
   Definition instr_aux : seal (@instr_def). by eexists. Qed.
   Definition instr := unseal instr_aux.
   Definition instr_eq : @instr = @instr_def :=
     seal_eq instr_aux.
 
   Definition instr_ctx (intrs : gmap addr (list trc)) : iProp Σ :=
-    ghost_map_auth heap_instrs_name 1 intrs.
+    instr_table intrs.
+
+  Definition extern_reg_def `{!heapG Σ} (r : string) : iProp Σ :=
+    ⌜¬ is_local_register r⌝.
+  Definition extern_reg_aux : seal (@extern_reg_def _). by eexists. Qed.
+  Definition extern_reg := unseal extern_reg_aux.
+  Definition extern_reg_eq : @extern_reg = @extern_reg_def _ :=
+    seal_eq extern_reg_aux.
 
   Definition reg_mapsto_def (γ : gname) (r : string) (q : frac) (v: valu) : iProp Σ :=
     r ↪[ γ ]{# q} v.
@@ -43,8 +68,20 @@ Section definitions.
   Definition regs_ctx `{!threadG} (regs : reg_map) : iProp Σ :=
     ghost_map_auth thread_regs_name 1 (reg_map_to_gmap regs).
 
+  Definition spec_trace_def (κs: list seq_label) : iProp Σ :=
+    ghost_var heap_spec_trace_name (1/2) κs.
+  Definition spec_trace_aux : seal (@spec_trace_def). by eexists. Qed.
+  Definition spec_trace := unseal spec_trace_aux.
+  Definition spec_trace_eq : @spec_trace = @spec_trace_def :=
+    seal_eq spec_trace_aux.
+
+  Definition spec_ctx (κs : list seq_label) : iProp Σ :=
+    ∃ κscur κsspec_end, ⌜heap_full_trace = κscur ++ κs⌝ ∗
+    ⌜heap_spec_trace = κscur ++ κsspec_end⌝ ∗
+    ghost_var heap_spec_trace_name (1/2) κsspec_end.
+
   Definition state_ctx (σ : seq_global_state) (κs : list seq_label) : iProp Σ :=
-    ⌜True⌝ ∗
+    spec_ctx κs ∗
     instr_ctx σ.(seq_instrs).
 
   Definition thread_ctx `{!threadG} (regs : reg_map) : iProp Σ :=
@@ -55,26 +92,56 @@ End definitions.
 Notation "r ↦ᵣ{ q } v" := (reg_mapsto thread_regs_name r q v)
   (at level 20, q at level 50, format "r  ↦ᵣ{ q }  v") : bi_scope.
 Notation "r ↦ᵣ v" := (reg_mapsto thread_regs_name r 1 v) (at level 20) : bi_scope.
+Notation "r ↦ᵣ !" := (extern_reg r) (at level 20) : bi_scope.
 
 Section instr.
   Context `{!heapG Σ}.
+  Global Instance instr_table_pers i : Persistent (instr_table i).
+  Proof. rewrite instr_table_eq. by apply _. Qed.
+
+  Global Instance instr_table_tl i : Timeless (instr_table i).
+  Proof. rewrite instr_table_eq. by apply _. Qed.
+
   Global Instance instr_pers a i : Persistent (instr a i).
   Proof. rewrite instr_eq. by apply _. Qed.
 
   Global Instance instr_tl a i : Timeless (instr a i).
   Proof. rewrite instr_eq. by apply _. Qed.
 
+  Lemma instr_table_agree i1 i2 :
+    instr_table i1 -∗ instr_table i2 -∗ ⌜i1 = i2⌝.
+  Proof.
+    rewrite instr_table_eq. iIntros "H1 H2".
+    iDestruct (own_valid_2 with "H1 H2") as %Hvalid.
+    move: Hvalid => /to_agree_op_valid.
+      by fold_leibniz.
+  Qed.
+
   Lemma instr_lookup instrs a i :
-    instr_ctx instrs -∗ instr a i -∗ ⌜instrs !! a = Some i⌝.
-  Proof. rewrite instr_eq. by apply ghost_map_lookup. Qed.
+    instr_ctx instrs -∗ instr a i -∗ ⌜instrs !! a = i⌝.
+  Proof.
+    rewrite instr_eq. iIntros "Htbl Hf".
+    iDestruct "Hf" as (i2 ?) "Hf".
+    by iDestruct (instr_table_agree with "Htbl Hf") as %->.
+  Qed.
 
 End instr.
 
 Section reg.
   Context `{!heapG Σ}.
 
+  Global Instance extern_reg_pers r : Persistent (r ↦ᵣ !).
+  Proof. rewrite extern_reg_eq. by apply _. Qed.
+
+  Global Instance extern_reg_tl r : Timeless (r ↦ᵣ !).
+  Proof. rewrite extern_reg_eq. by apply _. Qed.
+
   Global Instance reg_mapsto_tl γ r q v : Timeless (reg_mapsto γ r q v).
   Proof. rewrite reg_mapsto_eq. by apply _. Qed.
+
+  Lemma extern_reg_non_local r:
+    r ↦ᵣ ! -∗ ⌜¬ is_local_register r⌝.
+  Proof. by rewrite extern_reg_eq. Qed.
 
   Lemma reg_mapsto_lookup `{!threadG} regs r q v :
     regs_ctx regs -∗ r ↦ᵣ{q} v -∗ ⌜regs !! r = Some v⌝.
@@ -95,3 +162,25 @@ Section reg.
     by erewrite reg_map_to_gmap_insert.
   Qed.
 End reg.
+
+Section spec.
+  Context `{!heapG Σ}.
+
+  Global Instance spec_trace_tl κs : Timeless (spec_trace κs).
+  Proof. rewrite spec_trace_eq. by apply _. Qed.
+
+  Lemma spec_ctx_cons κ κs1 κs2:
+    spec_ctx (κ :: κs2) -∗ spec_trace (κ :: κs1) ==∗
+    spec_ctx κs2 ∗ spec_trace κs1.
+  Proof.
+    rewrite spec_trace_eq.
+    iDestruct 1 as (?? Hfull Hspec) "Hsc". iIntros "Hs".
+    iDestruct (ghost_var_agree with "Hsc Hs") as %?. subst.
+    iMod (ghost_var_update_halves with "Hsc Hs") as "[$ ?]".
+    iModIntro. iExists _, _. iFrame.
+    rewrite cons_middle app_assoc in Hfull.
+    rewrite cons_middle app_assoc in Hspec.
+    done.
+  Qed.
+
+End spec.
