theories/adequacy.v
@@ -1,0 +1,71 @@
+From iris.proofmode Require Import tactics.
+From iris.program_logic Require Export adequacy weakestpre.
+From iris.algebra Require Import csum excl auth cmra_big_op gmap.
+From iris.base_logic.lib Require Import ghost_map ghost_var.
+From isla Require Import ghost_state lifting.
+From iris.program_logic Require Export language.
+Set Default Proof Using "Type".
+
+Class islaPreG Σ := PreIslaG {
+  isla_pre_invG :> invPreG Σ;
+  heap_pre_instrs_inG :> inG Σ (instrtblUR);
+  heap_pre_regs_inG :> ghost_mapG Σ string valu;
+  heap_pre_spec_inG :> ghost_varG Σ (list seq_label);
+}.
+
+Definition islaΣ : gFunctors :=
+  #[invΣ; GFunctor (constRF instrtblUR); ghost_mapΣ string valu; ghost_varΣ (list seq_label)].
+
+Instance subG_islaPreG {Σ} : subG islaΣ Σ → islaPreG Σ.
+Proof. solve_inG. Qed.
+
+Definition initial_local_state (regs : reg_map) : seq_local_state := {|
+  seq_trace := [];
+  seq_regs := regs;
+  seq_nb_state := false;
+|}.
+
+Lemma isla_adequacy Σ `{!islaPreG Σ} (instrs : gmap addr (list trc)) (regs : list reg_map) κsspec t2 σ2 κs n:
+  (∀ {HG : islaG Σ},
+    ⊢ instr_table instrs -∗ spec_trace κsspec
+    ={⊤}=∗ [∗ list] rs ∈ regs, ∀ (_ : threadG), ([∗ map] r↦v∈reg_map_to_gmap rs, r ↦ᵣ v) -∗ WPasm []) →
+  nsteps n (initial_local_state <$> regs, {| seq_instrs := instrs |}) κs (t2, σ2) →
+  (∀ e2, e2 ∈ t2 → not_stuck e2 σ2) ∧
+  κs `prefix_of` κsspec.
+Proof.
+  move => Hwp.
+  apply: wp_strong_adequacy => ?.
+  set i := to_instrtbl instrs.
+  iMod (own_alloc (i)) as (γi) "#Hi" => //.
+  iMod (ghost_var_alloc κsspec) as (γs) "[Hs1 Hs2]".
+
+  set (HheapG := HeapG _ _ γi _ κs κsspec _ γs).
+  set (HislaG := IslaG _ _ HheapG).
+  iAssert (instr_table instrs) as "#His". { by rewrite instr_table_eq. }
+
+  iMod (Hwp HislaG with "His [Hs1]") as "Hwp". {
+    rewrite spec_trace_eq. iFrame.
+  }
+
+  iModIntro.
+  iExists NotStuck, _, (replicate (length regs) (λ _, True%I)), _, _.
+  iSplitL "Hs2"; last first; [iSplitL|].
+  - rewrite big_sepL2_replicate_r ?fmap_length // big_sepL_fmap.
+    iApply (big_sepL_impl with "Hwp").
+    iIntros "!>" (? rs ?) "Hwp".
+    iMod (ghost_map_alloc (reg_map_to_gmap rs)) as (γr) "[Hr1 Hr2]".
+    set (HthreadG := ThreadG γr).
+    setoid_rewrite wp_asm_unfold.
+    iApply ("Hwp" with "[Hr2]"); [|done|done|done].
+    iApply (big_sepM_impl with "Hr2").
+    iIntros "!>" (???) "?".
+      by rewrite reg_mapsto_eq.
+  - iIntros (?????) "(Hspec&?) ? ?".
+    iApply fupd_mask_intro; [done|]. iIntros "_".
+    iDestruct "Hspec" as (? ? Hκs Hspec) "?".
+    simpl in *. subst.
+    iPureIntro. split; [naive_solver|].
+    rewrite right_id. by apply: prefix_app_r.
+  - simpl. iFrame "His".
+    iExists [], _. by iFrame.
+Qed.
