README.md
@@ -11,6 +11,7 @@ following commands:
 opam switch create . ocaml-base-compiler.4.11.1
 opam repo add coq-released https://coq.inria.fr/opam/released
 opam repo add iris-dev https://gitlab.mpi-sws.org/iris/opam.git
+opam pin add -n -y cerberus "git+https://github.com/rems-project/cerberus.git#9f3a825a5f32a8245101a57105a5598a1adf6879"
 make builddep
 ```
 
